\documentclass[12pt]{article}
\usepackage[utf8]{inputenc}
\usepackage{float}
\usepackage{amsmath}

\usepackage[hmargin=3cm,vmargin=6.0cm]{geometry}
%\topmargin=0cm
\topmargin=-2cm
\addtolength{\textheight}{6.5cm}
\addtolength{\textwidth}{2.0cm}
%\setlength{\leftmargin}{-5cm}
\setlength{\oddsidemargin}{0.0cm}
\setlength{\evensidemargin}{0.0cm}

%misc libraries goes here
\usepackage{amssymb}
\newcommand{\divides}{\mid}
\newcommand{\notdivides}{\nmid}
\newcommand{\Mod}[1]{\ (\mathrm{mod}\ #1)}
\newcommand{\+}{\mkern2mu}
\newcommand{\uq}[1]{\forall #1}
\newcommand{\eq}[1]{\exists \+ #1}
\newcommand{\bb}[1]{\mathbb{#1}}

\begin{document}

\section*{Student Information }
%Write your full name and id number between the colon and newline
%Put one empty space character after colon and before newline
Full Name : Murat Bolu \\
Id Number : 2521300 \\

% Write your answers below the section tags
\section*{Answer 1}

\begin{description}
    \item[Basis:] For $n = 1$, $6^{2n} - 1 = 6^2 - 1 = 35$, and $5 \divides 35$, and $7 \divides 35$.
    \item[Inductive Step:] Assuming that $6^{2n} - 1$ is divisible by both $5$ and $7$, one can show that $6^{2(n+1)} - 1 = 6^{2n+2} - 1$ is divisible by $5$ and $7$ for $n \in \{1, 2, 3, \dotsc\}$. Since $5 \divides 6^{2n} - 1$ and $7 \divides 6^{2n} - 1$, that means $35 \divides 6^{2n} - 1$ which is shown below.
    \begin{align*}
        6^{2n} - 1 &= 5 \cdot x && \text{for some $x \in \mathbb{N}$} \\
        6^{2n} - 1 &= 7 \cdot y && \text{for some $y \in \mathbb{N}$} \\
        5 \cdot x &= 7 \cdot y
    \end{align*}
    Since $x$ and $y$ are natural numbers, $x$ must be divisible by $7$ and $y$ must be divisible by $5$, and we can rewrite them as $x = 7 \cdot k$ and $y = 5 \cdot l$. The other possibility is that they are both zero, which is obviously not possible since $6^{2n} - 1$ is at least $35$.
    \begin{align*}
        6^{2n} - 1 &= 5 \cdot 7 \cdot k && \text{for some $k \in \mathbb{N}$} \\
        6^{2n} - 1 &= 7 \cdot 5 \cdot l && \text{for some $l \in \mathbb{N}$} \\
        6^{2n} - 1 &= 35 \cdot k \\
        6^{2n} - 1 &= 35 \cdot l
    \end{align*}
    There exists $k$ or $l$ such that they are natural numbers, and that means $6^{2n} - 1$ is divisible by $35$.
    \begin{align*}
        6^{2n} - 1 &\equiv 0 && \Mod{35} \\
        6^{2n} &\equiv 1 && \Mod{35} \\
        6^{2n+2} &\equiv 36 && \Mod{35} \\
        6^{2n+2} &\equiv 1 && \Mod{35} \\
        6^{2n+2} - 1 & \equiv 0 && \Mod{35}
    \end{align*}
    Therefore, there exists a natural number $a \in \mathbb{N}$ such that $6^{2n+2} - 1 = 35 \cdot a$. It is obvious that $6^{2n+2} - 1$ is divisible by both $5$ and $7$ since $5 \divides 35a$ and $7 \divides 35a$.

    \hfill $\blacksquare$
\end{description}

\newpage

\section*{Answer 2}

\begin{description}
    \item[Basis:]
    \begin{itemize}
        \item[]
        \item For $n = 0$, $H_0 = 1 \leq 1 = 9^0$.
        \item For $n = 1$, $H_1 = 5 \leq 9 = 9^1$.
        \item For $n = 2$, $H_2 = 7 \leq 81 = 9^2$.
        \item For $n = 3$, $H_3 = 8H_2 + 8H_1 + 9H_0 = 8 \cdot 7 + 8 \cdot 5 + 9 \cdot 1 = 105 \leq 729 = 9^3$.
    \end{itemize}
    \item[Inductive Step:] Assuming that $H_n \leq 9^n$, $\uq{n} \leq k$, one can show that $H_{k+1}$ is less than or equal to $9^{k+1}$. We can replace every $H_n$ with something greater than or equal to itself.
    \begin{align*}
        H_{k+1} &= 8H_k + 8H_{k-1} + 9H_{k-2} \\
        H_{k+1} &\leq 8 \cdot 9^k + 8H_{k-1} + 9H_{k-2} \\
        H_{k+1} &\leq 8 \cdot 9^k + 8 \cdot 9^{k-1} + 9H_{k-2} \\
        H_{k+1} &\leq 8 \cdot 9^k + 8 \cdot 9^{k-1} + 9 \cdot 9^{k-2} \\
        H_{k+1} &\leq 8 \cdot 9^k + 8 \cdot 9^{k-1} + 9^{k-1} \\
        H_{k+1} &\leq 8 \cdot 9^k + 9 \cdot 9^{k-1} \\
        H_{k+1} &\leq 8 \cdot 9^k + 9^{k} \\
        H_{k+1} &\leq 9 \cdot 9^k \\
        H_{k+1} &\leq 9^{k+1}
    \end{align*}

    \hfill $\blacksquare$
\end{description}

\section*{Answer 3}

Let $A$ denote the set that contains 8 digit bit strings that contain four consecutive zeros and $B$ denote the set that contains 8 digit bit strings that contain four consecutive ones. It it clear that the answer we are looking for is $|A \cup B|$ which is equal to the commonly known identity $|A| + |B| - |A \cap B|$. It can be seen that $A \cap B = \{00001111, 11110000\}$ and $|A \cap B| = 2$. Then, we need to find $|A|$ and $|B|$.
\newline
Let $a_n$ denote the number of strings of size $n$ that contain four consecutive zeros and $b_n$ denote the number of strings of size $n$ that contain four consecutive ones. One can see that $|A| = a_8$ and $|B| = b_8$.
\newline
$a_n$ can be written as a recurrence relation where $a_n = 2 \cdot a_{n-1} + 2^{n-5} - a_{n-5}$ and $a_0 = a_1 = a_2 = a_3 = 0$, $a_4 = 1$. The initial conditions are obvious, and the reason for recurrence relation is that we can append zero or one to a valid digit of size $n - 1$ to get a valid digit of size $n$, hence $2 \cdot a_{n-1}$. We can also take a invalid digit of size $n - 5$ and append $10000$ to it, invalid digits are all digits minus the valid digits, hence $2^{n-5} - a_{n-5}$. One can calculate $a_5 = 3$, $a_6 = 8$, $a_7 = 20$, and $a_8 = 48$.
\newline
The same argument applies to $b_n$ where the bits are flipped, so $b_8 = 48$. Therefore $|A| = 48$, $|B| = 48$, and $|A \cup B| = 48 + 48 - 2 = 94$.

\section*{Answer 4}

\section*{Answer 5}
\paragraph{a)}
\paragraph{b)}
\paragraph{c)}

\end{document}
